StrataTest/DL/Imperative/Arith.lean
@@ -19,9 +19,9 @@ def typeCheckAndPartialEval (cmds : Commands) : Except Format (Commands × Eval.
   return (cmds, S)
 
 private def testProgram1 : Commands :=
-  [.init "x" .Num (some (.Var "y" (.some .Num))),
-   .havoc "x",
-   .assert "x_value_eq" (.Eq (.Var "x" .none) (.Var "y" none))]
+  [.init "x" .Num (some (.Var "y" (.some .Num))) .empty,
+   .havoc "x" .empty,
+   .assert "x_value_eq" (.Eq (.Var "x" .none) (.Var "y" none)) .empty]
 
 /--
 info: ok: Commands:
@@ -48,9 +48,9 @@ genNum: 1
 
 
 private def testProgram2 : Commands :=
-  [.init "x" .Num (some (.Num 0)),
-   .set "x" (.Plus (.Var "x" .none) (.Num 100)),
-   .assert "x_value_eq" (.Eq (.Var "x" .none) (.Num 100))]
+  [.init "x" .Num (some (.Num 0)) .empty,
+   .set "x" (.Plus (.Var "x" .none) (.Num 100)) .empty,
+   .assert "x_value_eq" (.Eq (.Var "x" .none) (.Num 100)) .empty]
 
 /--
 info: ok: Commands:
