StrataTest/Languages/C_Simp/Examples/LoopSimple.lean
@@ -79,7 +79,7 @@ info: function loopSimple {
 }
 -/
 #guard_msgs in
-#eval Strata.C_Simp.get_program LoopSimplePgm
+#eval (Strata.C_Simp.get_program LoopSimplePgm).stripMetaData
 
 /--
 info: procedure loopSimple (n : int) returns (return : int)
