StrataTest/Languages/Core/Examples/TypeDecl.lean
@@ -119,7 +119,7 @@ type int := bool;
 #end
 
 /--
-error: (0,(0-0)) ❌ Type checking error.
+error:  ❌ Type checking error.
 This type declaration's name is reserved!
 int := bool
 KnownTypes' names:
