StrataTest/Languages/Core/ProcedureEvalTests.lean
@@ -238,7 +238,7 @@ Proof Obligation:
                     preconditions := [("0_lt_x", ⟨eb[((~Int.Lt #0) x)], .Default, #[]⟩)],
                     postconditions := [("ret_y_lt_0", ⟨eb[((~Int.Lt y) #0)], .Default, #[]⟩)] },
                 body := [
-                  Statement.set "y" eb[(~Int.Neg x)]
+                  Statement.set "y" eb[(~Int.Neg x)] .empty
                 ]
               }
           return format E
